Added tactics to unfold method specs

Java/src/Java/Examples/ListClass.v
@@ -10,9 +10,18 @@ Require Import Java.Semantics.OperationalSemantics.
 Require Import Java.Logic.AssertionLogic.
 Require Import Java.Logic.SpecLogic.
 Require Import Java.Examples.ListModel.
+Require Import Java.Func.Reify.
+Require Import Java.Func.JavaFunc.
+Require Import Java.Func.Type.
+Require Import Java.Tactics.SymEx.
+Require Import Java.Tactics.Tactics.
 
 Require Import Coq.Lists.List.
 Require Import Coq.Strings.String.
+
+Require Import ExtLib.Structures.Applicative.
+Require Import MirrorCore.TypesI.
+Require Import ChargeCore.Open.OpenILogic.
 
 Set Implicit Arguments.
 Unset Strict Implicit.
@@ -45,7 +54,7 @@ Definition cons_body :=
                           (cwrite "this" "head" (E_var "n")))))).
 
 Definition ConsM : Method :=
-  Build_Method ("this"::"n"::nil) cons_body (E_val null).
+  Build_Method ("this"::"x"::nil) cons_body (E_val null).
 
 Definition reverse_body :=
   (cseq (cread "i" "this" "head")
@@ -70,23 +79,20 @@ Definition ListC := Build_Class ("head"::nil) (("head", HeadM) ::
                                                nil).
 
 Definition ListProg := Build_Program
-                         (("List", ListC)::("Node", NodeC)::nil).  
+                         (("List", ListC)::("Node", NodeC)::nil).
+                         
 
-Require Import ExtLib.Structures.Applicative.
-Require Import MirrorCore.TypesI.
-Require Import ChargeCore.Open.OpenILogic.
-
-Local Instance Applicative_Fun : Applicative (RFun stack) :=
+Local Instance Applicative_Fun : Applicative (RFun (string -> val)) :=
 { pure := fun _ x _ => x
 ; ap := fun _ _ f x y => (f y) (x y)
 }.
 
 Definition head_frame x xs : sasn :=
-  (ap (ap (pure (T := RFun stack) List) 
+  (ap (ap (pure (T := RFun (string -> val)) List) 
           (stack_get "this")) 
-      (pure  (T := RFun stack) (x::xs))).
+      (pure  (T := RFun (string -> val)) (x::xs))).
 Definition head_return x : sasn := 
-    (embed (open_eq (stack_get "r") (pure (T := RFun stack) x))).
+    (embed (open_eq (stack_get "r") (pure (T := RFun (string -> val)) x))).
 Definition head_requires x xs := head_frame x xs.
 Definition head_ensures x xs := head_frame x xs.
 
@@ -99,29 +105,29 @@ Definition head_spec : spec :=
 
 
 Definition tail_frame h n : sasn :=
-  ap (ap (ap (pure (T := RFun stack) pointsto) 
+  ap (ap (ap (pure (T := RFun (string -> val)) pointsto) 
              (stack_get "this"))
-         (pure (T := RFun stack) "head"))
-     (pure (T := RFun stack) h) ** 
-  ap (ap (ap (pure (T := RFun stack) pointsto) 
-             (pure (T := RFun stack) h))
-         (pure (T := RFun stack) "next"))
-     (pure (T := RFun stack) n).
+         (pure (T := RFun (string -> val)) "head"))
+     (pure (T := RFun (string -> val)) h) ** 
+  ap (ap (ap (pure (T := RFun (string -> val)) pointsto) 
+             (pure (T := RFun (string -> val)) h))
+         (pure (T := RFun (string -> val)) "next"))
+     (pure (T := RFun (string -> val)) n).
 Definition tail_return n : sasn := 
-    (embed (open_eq (stack_get "r") (pure (T := RFun stack) n))).
+    (embed (open_eq (stack_get "r") (pure (T := RFun (string -> val)) n))).
 Definition tail_requires h n xs : sasn :=
   tail_frame h n **
-  ap (ap (pure (T := RFun stack) Node) 
+  ap (ap (pure (T := RFun (string -> val)) Node) 
          (stack_get "this"))
-     (pure  (T := RFun stack) xs).
+     (pure  (T := RFun (string -> val)) xs).
 Definition tail_ensures h n xs : sasn :=
   tail_frame h n **
-  ap (ap (pure (T := RFun stack) List) 
+  ap (ap (pure (T := RFun (string -> val)) List) 
           (stack_get "this")) 
-     (pure  (T := RFun stack) xs).
+     (pure  (T := RFun (string -> val)) xs).
 
 Definition tail_spec : spec :=
-  Forall h : val, Forall n : val, Forall x : val, Forall xs : list val, 
+  Forall h : val, Forall n : val, Forall xs : list val, 
     method_spec "List" "tail" ("this"::nil) "r"
                 (tail_requires h n xs)
                 (tail_ensures h n xs //\\ tail_return n).
@@ -129,15 +135,15 @@ Definition tail_spec : spec :=
 
 
 Definition cons_requires xs : sasn :=
-  ap (ap (pure (T := RFun stack) List) 
+  ap (ap (pure (T := RFun (string -> val)) List) 
          (stack_get "this")) 
-     (pure  (T := RFun stack) xs).
+     (pure  (T := RFun (string -> val)) xs).
 Definition cons_ensures xs : sasn :=
   ap (ap (pure List) 
          (stack_get "this")) 
      (ap (ap (pure cons) 
              (stack_get "n")) 
-         (pure (T := RFun stack) xs)).
+         (pure (T := RFun (string -> val)) xs)).
                                             
 Definition cons_spec : spec :=
     Forall xs : list val, 
@@ -148,27 +154,83 @@ Definition cons_spec : spec :=
 
 
 Definition reverse_requires xs : sasn :=
-  ap (ap (pure (T := RFun stack) List) 
+  ap (ap (pure (T := RFun (string -> val)) List) 
          (stack_get "this")) 
-     (pure  (T := RFun stack) xs).
+     (pure  (T := RFun (string -> val)) xs).
 Definition reverse_ensures xs : sasn :=
-  ap (ap (pure (T := RFun stack) List) 
+  ap (ap (pure (T := RFun (string -> val)) List) 
          (stack_get "this")) 
-     (pure  (T := RFun stack) (rev xs)).
+     (pure  (T := RFun (string -> val)) (rev xs)).
 
 Definition reverse_spec : spec :=
     Forall xs : list val, 
       method_spec "List" "reverse" ("this"::nil) "" 
                   (reverse_requires xs)
                   (reverse_ensures xs).
-            
-Lemma HeadCorrect : prog_eq ListProg |-- head_spec.
+
+Lemma unfold_method_spec (C : class) (m : string) 
+  (pn pn' : list Lang.var) (rn : Lang.var) (Pr : Program) P Q c re S
+  (HS : S |-- prog_eq Pr)
+  (HNoDup : NoDup (rn::pn)) 
+  (HSpec : method_lookup Pr C m {| m_params := pn'; m_body := c; m_ret := re |}) 
+  (Hlength : Datatypes.length pn = Datatypes.length pn') 
+  (Hmodify : forall x : Lang.var, In x pn' -> ~ In x (modifies c)) 
+  (Htriple : S |-- triple (Subst.apply_subst P
+          (Subst.substl_trunc (combine pn (map Open.var_expr pn')))) 
+          (Subst.apply_subst Q
+          (Subst.substl_trunc
+            (combine (rn :: pn) (eval re :: map Open.var_expr pn')))) c) : 
+   S |-- method_spec C m pn rn P Q.
 Proof.
-  admit.
-Admitted.
+  unfold method_spec.
+  repeat (apply lforallR; intros).
+  apply landR. 
+  apply embedPropR; assumption.
+  apply (lexistsR pn').
+  apply (lexistsR c).
+  apply (lexistsR re).
+  apply landR.
+  etransitivity; [apply HS|]; apply prog_eq_to_prop.
+  repeat split; assumption.
+  assumption.
+Qed.
+
+Ltac solve_NoDup :=
+  repeat (apply NoDup_cons; simpl); 
+    first [intuition congruence | apply NoDup_nil].
+
+Ltac solve_method_lookup :=
+  unfold method_lookup; eexists; split; simpl; [
+    intuition congruence|]; simpl; intuition congruence.
+    
+Ltac solve_subst :=
+  run_rtac reify_java term_table substTac2_sound.
+
+Opaque embed.
+Opaque ap.
+Opaque pure.
+
+Instance fs : Environment := 
+  Build_Environment (FMapPositive.PositiveMap.empty (SymEnv.function typ _)).
+
 
 Lemma TailCorrect : prog_eq ListProg |-- tail_spec.
 Proof.
+  unfold tail_spec. unfold tail_requires. 
+  unfold tail_ensures. unfold tail_return.
+  repeat (apply lforallR; intros).
+  eapply unfold_method_spec; [
+    reflexivity |
+    solve_NoDup |
+    solve_method_lookup |
+    simpl; reflexivity |
+    simpl; intuition congruence |
+    simpl
+  ].
+    unfold tail_frame.
+    unfold Lang.var.
+    revert x; revert x0; revert x1.
+    solve_subst.
   admit.
 Admitted.
 
