Java/src/Java/Examples/Swap.v
@@ -1,0 +1,162 @@
+Require Import ChargeCore.Logics.ILogic.
+Require Import ChargeCore.Logics.BILogic.
+Require Import ChargeCore.Logics.ILEmbed.
+Require Import ChargeCore.Open.Stack.
+
+Require Import Java.Language.Lang.
+Require Import Java.Language.Program.
+Require Import Java.Semantics.AxiomaticSemantics.
+Require Import Java.Semantics.OperationalSemantics.
+Require Import Java.Logic.AssertionLogic.
+Require Import Java.Logic.SpecLogic.
+Require Import Java.Func.Reify.
+Require Import Java.Func.JavaFunc.
+Require Import Java.Func.Type.
+Require Import Java.Tactics.SymEx.
+Require Import Java.Tactics.Tactics.
+
+Require Import Coq.Lists.List.
+Require Import Coq.Strings.String.
+Require Import Coq.Numbers.BinNums.
+Require Import ExtLib.Structures.Applicative.
+Require Import MirrorCore.TypesI.
+Require Import MirrorCore.Lambda.ExprDsimul.
+Require Import ChargeCore.Open.OpenILogic.
+
+Open Scope string.
+
+Local Instance Applicative_Fun : Applicative (RFun (String.string -> val)) := 
+{ pure := fun _ x _ => x
+; ap := fun _ _ f x y => (f y) (x y)
+}.
+
+(* Swap represents type Swap *)
+Module Swap.
+Definition x : field := "x".
+Definition y : field := "y".
+
+Definition C : string := "Swap"%string.
+Definition T : Type := (val * val).
+Definition Swap := (fun p xy => (pointsto p x (fst xy)) ** (pointsto p y (snd xy))).
+
+(* Start of specifications for set_int_int_void known as set_int_int_void *)
+
+(* set_int_int_void body *)
+Definition set_int_int_void_function := fun (t:T) (x:val) (y:val) => ((x,y),nothing).
+
+Definition set_int_int_void_body :=
+	(cseq (cwrite ("this")%string ("x")%string (E_var ("x_new")%string)) (cwrite ("this")%string ("y")%string (E_var ("y_new")%string))).
+
+Definition nothing := (vint 0).
+
+(* set_int_int_void definition *)
+Definition set_int_int_void_method :=
+	(Build_Method (("this")%string :: (("x_new")%string :: (("y_new")%string :: nil))) set_int_int_void_body (E_val nothing)).
+
+(* Specification for set_int_int_void *)
+Definition set_int_int_void_requires (t : (val * val)) : sasn :=
+	ltrue ** (ap (ap (pure (T := RFun (String.string -> val)) Swap) (stack_get ("this")%string)) (pure (T := RFun (String.string -> val)) t)).
+
+(* Specification for set_int_int_void *)
+Definition set_int_int_void_ensures : sasn :=
+	ltrue ** (ap (ap (pure (T := RFun (String.string -> val)) Swap) (stack_get ("this")%string)) (ap (ap (pure (T := RFun (String.string -> val)) pair) (stack_get ("x_new")%string)) (stack_get ("y_new")%string))).
+
+(* set_int_int_void specification *)
+Definition set_int_int_void_spec : spec :=
+	Forall t : (val * val), (method_spec (C)%string ("set_int_int_void")%string (("this")%string :: (("x_new")%string :: (("y_new")%string :: nil))) ("")%string (set_int_int_void_requires t) (set_int_int_void_ensures //\\ ltrue)).
+
+(* Start of specifications for swap_void known as swap_void *)
+
+(* swap_void body *)
+Definition swap_void_function := fun xy:T => ((snd (xy),fst (xy)), nothing).
+
+Definition swap_void_body :=
+	(cseq (cread ("x_old")%string ("this")%string ("x")%string) (cseq (cread ("y_old")%string ("this")%string ("y")%string) (cseq (cwrite ("this")%string ("x")%string (E_var ("y_old")%string)) (cwrite ("this")%string ("y")%string (E_var ("x_old")%string))))).
+
+(* swap_void definition *)
+Definition swap_void_method :=
+	(Build_Method (("this")%string :: nil) swap_void_body (E_val nothing)).
+
+(* Specification for swap_void *)
+Definition swap_void_requires (x : (val)) (y : (val)) : sasn :=
+	ltrue ** (ap (ap (pure (T := RFun (String.string -> val)) Swap) (stack_get ("this")%string)) (ap (ap (pure (T := RFun (String.string -> val)) pair) (pure (T := RFun (String.string -> val)) x)) (pure (T := RFun (String.string -> val)) y))).
+
+(* Specification for swap_void *)
+Definition swap_void_ensures (x : (val)) (y : (val)) : sasn :=
+	ltrue ** (ap (ap (pure (T := RFun (String.string -> val)) Swap) (stack_get ("this")%string)) (ap (ap (pure (T := RFun (String.string -> val)) pair) (pure (T := RFun (String.string -> val)) y)) (pure (T := RFun (String.string -> val)) x))).
+
+(* swap_void specification *)
+Definition swap_void_spec : spec :=
+	Forall x : (val), Forall y : (val), (method_spec (C)%string ("swap_void")%string (("this")%string :: nil) ("")%string (swap_void_requires x y) (swap_void_ensures x y //\\ ltrue)).
+
+(* Class spec for Swap *)
+Definition Class_spec :=
+	(Build_Class (("x")%string :: (("y")%string :: nil)) ((("set_int_int_void")%string, set_int_int_void_method) :: ((("swap_void")%string, swap_void_method) :: nil))).
+
+End Swap.
+
+Definition Swap_prog :=
+	(Build_Program (((Swap.C)%string, Swap.Class_spec) :: nil)).
+ 
+ 
+Module Theorems.
+
+Instance fs : Environment := 
+  Build_Environment (FMapPositive.PositiveMap.empty (SymEnv.function typ _)).
+
+(* set_int_int_void correctness lemma *)
+Opaque ap.
+Opaque pure.
+
+Lemma set_int_int_void_correct : prog_eq Swap_prog |-- Swap.set_int_int_void_spec.
+Proof.
+  unfold Swap.set_int_int_void_spec.
+  unfold Swap.set_int_int_void_requires.
+  unfold Swap.set_int_int_void_ensures.
+  unfold Swap.Swap.
+  apply lforallR.
+  intros t.
+  unfold_method_spec.
+  revert t.
+  run_rtac reify_java term_table substTac2_sound.
+Qed.
+
+(* swap_void correctness lemma *)
+Lemma swap_void_correct : prog_eq Swap_prog |-- Swap.swap_void_spec.
+Proof.  
+  unfold Swap.swap_void_spec.
+  unfold method_spec.
+  apply lforallR.
+  intros.
+  rename x into t_x.
+  apply lforallR.
+  intros.
+  rename x into t_y.
+  apply landR.
+  - apply embedPropR.
+    apply nodup_sound.
+    reflexivity. 
+  - apply lexistsR with (x := (("this")%string :: nil)).
+    apply lexistsR with (x := (cseq (cread ("x_old")%string ("this")%string ("x")%string) (cseq (cread ("y_old")%string ("this")%string ("y")%string) (cseq (cwrite ("this")%string ("x")%string (E_var ("y_old")%string)) (cwrite ("this")%string ("y")%string (E_var ("x_old")%string)))))).
+    apply lexistsR with (x := E_val nothing).
+ 	apply landR.
+    + apply prog_eq_to_prop.
+      split.
+      * unfold method_lookup.
+        exists Swap.Class_spec.
+        split.
+        -- simpl. left. reflexivity.
+        -- simpl. right. left. unfold Swap.swap_void_method. unfold Swap.swap_void_body. reflexivity.
+      * split.
+        -- reflexivity.
+        -- unfold not. intros. simpl in *. intuition congruence.
+    + admit.  
+Admitted.
+
+(* Swap correctness theorem *)
+Theorem Swap_correct : prog_eq Swap_prog |-- Swap.set_int_int_void_spec //\\ Swap.swap_void_spec.
+Proof.
+Admitted.
+
+End Theorems.
+
